Added a Swap gate, aliased ZX_CNOT_is_cnot to ZX_CNOT_l_is_cnot per convention, proved ZX_SWAP_is_swap.

Gates.v
@@ -30,3 +30,20 @@ Definition ZX_S : ZX 1 1 := Z_Spider 1 1 (PI / 2).
 Definition ZX_T : ZX 1 1 := Z_Spider 1 1 (PI / 4).
 
 Notation ZX_CNOT := ZX_CNOT_l.
+
+Definition ZX_FLIPPED_CNOT := 
+    (Compose 
+        (Stack
+            Wire 
+            (Z_Spider 1 2 0%R)) 
+        (Stack  
+            (X_Spider 2 1 0%R)
+            Wire)).
+
+
+Definition ZX_SWAP : ZX 2 2 :=
+    (Compose 
+        ZX_CNOT
+        (Compose 
+            ZX_FLIPPED_CNOT
+            ZX_CNOT)).
